Add new theorems to deal with synchronous `chor` transitions

semantics/semBakeryScript.sml
@@ -526,6 +526,9 @@ Proof
   >> fs[] >> metis_tac[]
 QED
 
+(* Transitions preserve ‘no_undefined_vars’ since they can not remove
+   variables from the state
+*)
 Theorem no_undefined_vars_trans_pres:
   ∀sc alpha sc'. no_undefined_vars sc ∧ trans sc alpha sc' ⇒ no_undefined_vars sc'
 Proof
@@ -541,6 +544,42 @@ Proof
   >> fs[SUBSET_DEF,INSERT_DEF,DIFF_DEF] >> metis_tac[]
 QED
 
+(* A tag does not remove variables from the state, hence preserving
+   ‘no_undefined_vars_def’
+*)
+Theorem no_undefined_vars_from_tags:
+  ∀c s α.
+   no_undefined_vars (s,c) ⇒ no_undefined_vars (state_from_tag s α, c)
+Proof
+  rw [no_undefined_vars_def,free_variables_def]
+  \\ Cases_on `α` \\ fs [state_from_tag_def]
+  \\ ho_match_mp_tac SUBSET_TRANS
+  \\ metis_tac [SUBSET_OF_INSERT]
+QED
+
+(* If there are no undefined variables no lookup into
+   the state should fail (give NONE)
+*)
+Theorem no_undefined_FLOOKUP:
+  (∀p v s c q x. no_undefined_vars (s,Com p v q x c)
+    ⇒ ∃x. FLOOKUP s (v,p) = SOME x)
+∧ (∀p v s c c1 c2. no_undefined_vars (s,IfThen v p c1 c2)
+    ⇒ ∃x. FLOOKUP s (v,p) = SOME x)
+∧ (∀p l s c v f. no_undefined_vars (s,Let v p f l c)
+    ⇒ EVERY IS_SOME (MAP (FLOOKUP s) (MAP (λv. (v,p)) l)))
+Proof
+  rw [no_undefined_vars_def,free_variables_def,FDOM_FLOOKUP]
+  \\ Induct_on ‘l’ \\ fs [] \\ rw [FDOM_FLOOKUP] \\ rw [IS_SOME_DEF]
+QED
+
+(* MP-friendly version of no_undefined_FLOOKUP *)
+val t_list = no_undefined_FLOOKUP |> CONJUNCTS
+
+Theorem no_undefined_FLOOKUP_if  = el 2 t_list
+Theorem no_undefined_FLOOKUP_com = el 1 t_list
+Theorem no_undefined_FLOOKUP_let = el 3 t_list
+
+(* Ensure no self communication of a choreography *)
 Definition no_self_comunication_def:
   no_self_comunication (Com p _ q _ c)   = (p ≠ q ∧ no_self_comunication c)
 ∧ no_self_comunication (Sel p _ q c)     = (p ≠ q ∧ no_self_comunication c)
@@ -549,5 +588,160 @@ Definition no_self_comunication_def:
 ∧ no_self_comunication (Let _ _ _ _ c)   = no_self_comunication c
 ∧ no_self_comunication _                 = T
 End
+
+(* Check if a tag matches the head of a choreography *)
+Definition chor_match_def:
+  chor_match (LCom p v q x)  (Com p' v' q' x' c)  = ((p,v,q,x)  = (p',v',q',x'))
+∧ chor_match (LSel p b q)    (Sel p' b' q' c)     = ((p,b,q)  = (p',b',q'))
+∧ chor_match (LLet v p f l)  (Let v' p' f' l' c)  = ((v,p,f,l) = (v',p',f',l'))
+∧ chor_match (LTau p v)      (IfThen v' p' c1 c2) = ((p,v)     = (p',v'))
+∧ chor_match  _              _                    = F
+End
+
+(* Generates the corresponding tag that would consume
+   the front of the choreography
+*)
+Definition chor_tag_def:
+  chor_tag (Com p v q x _)  = LCom p v q x
+∧ chor_tag (Sel p b q _)    = LSel p b q
+∧ chor_tag (Let v p f l _)  = LLet v p f l
+∧ chor_tag (IfThen v p _ _) = LTau p v
+End
+
+
+(* Drops the head of the choreography updating the state in the process.
+   Its equivalent to one synchronous step in the semantics.
+*)
+Definition chor_tl_def:
+  chor_tl s astBakery$Nil   = (s,astBakery$Nil)
+∧ chor_tl s (Com p v q x c) = (s |+ ((x,q),(THE o FLOOKUP s) (v,p)),c)
+∧ chor_tl s (Sel p b q c)   = (s,c)
+∧ chor_tl s (Let v p f l c) =
+    (s |+ ((v,p),f(MAP (THE o FLOOKUP s) (MAP (λv. (v,p)) l))),c)
+∧ chor_tl s (IfThen v p c1 c2) =
+    (if FLOOKUP s (v,p) = SOME [1w] then (s,c1)
+     else if ∃w. FLOOKUP s (v,p) = SOME w ∧ w ≠ [1w] then (s,c2)
+     else (s,IfThen v p c1 c2))
+End
+
+(* Advances the choreography until the given tag
+   matches removing everything in its path
+   (state is still updated)
+*)
+Definition syncTrm_def:
+  syncTrm (s,Nil) τ            = (s,Nil)
+∧ syncTrm (s,IfThen v p c1 c2) τ =
+   (if chor_match τ (IfThen v p c1 c2)
+    then chor_tl s (IfThen v p c1 c2)
+    else if FLOOKUP s (v,p) = SOME [1w]
+         then syncTrm (s,c1) τ
+         else if ∃w. FLOOKUP s (v,p) = SOME w ∧ w ≠ [1w]
+              then syncTrm (s,c2) τ
+              else (s,IfThen v p c1 c2))
+∧ syncTrm (s,c) τ =
+          (if chor_match τ c
+           then chor_tl s c
+           else syncTrm (chor_tl s c) τ)
+Termination
+  WF_REL_TAC ‘measure (chor_size o SND o FST)’
+  \\ rw [] \\ Cases_on ‘τ’ \\ fs [chor_match_def,chor_tl_def]
+  \\ EVERY_CASE_TAC  \\ fs []
+End
+
+(* Alternative induction principle *)
+Theorem syncTrm_pairind =
+  syncTrm_ind
+  |> Q.SPEC ‘λ(s,c) τ. P s c τ’
+  |> SIMP_RULE std_ss []
+  |> Q.GEN ‘P’
+
+(* A choreography can always advance synchronously consuming
+   the operation at the front
+*)
+Theorem chor_tag_trans:
+  ∀s c.
+   no_undefined_vars (s,c) ∧ c ≠ Nil
+   ∧ no_self_comunication c
+   ⇒ trans (s,c) (chor_tag c,[]) (syncTrm (s,c) (chor_tag c))
+Proof
+  rw [] \\ Cases_on ‘c’
+  \\ fs [ chor_tag_def,syncTrm_def,chor_match_def
+        , chor_tl_def,no_self_comunication_def]
+  >- (Cases_on ‘FLOOKUP s (s',l) = SOME [1w]’
+     >- fs [theorem"trans_if_true"]
+     \\ drule no_undefined_FLOOKUP_if \\ rw [] \\ fs []
+     \\ fs [theorem"trans_if_false"])
+  >- (drule no_undefined_FLOOKUP_com \\ rw []
+     \\  fs [theorem"trans_com"])
+  >- (drule no_undefined_FLOOKUP_let \\ rw []
+     \\  fs [theorem"trans_let"])
+  \\ fs [theorem"trans_sel"]
+QED
+
+(* A synchronous version of ‘trans_s’ *)
+Definition trans_sync_def:
+  trans_sync = RTC (λp q. ∃τ. trans p (τ,[]) q)
+End
+
+(* Basic RTC rules (reflexivity) *)
+Theorem trans_sync_refl:
+  ∀p. trans_sync p p
+Proof
+  rw [trans_sync_def,RTC_RULES]
+QED
+
+(* Basic RTC rules (single step) *)
+Theorem trans_sync_step:
+  ∀p p' τ q. trans p (τ,[]) p' ∧ trans_sync p' q ⇒ trans_sync p q
+Proof
+  rw [trans_sync_def] \\ ho_match_mp_tac RTC_TRANS
+  \\ qexists_tac ‘p'’ \\ rw []
+  \\ asm_exists_tac \\ fs []
+QED
+
+(* Basic RTC rules (transitivity) *)
+Theorem trans_sync_trans:
+  ∀p p' q. trans_sync p p' ∧ trans_sync p' q ⇒ trans_sync p q
+Proof
+  metis_tac [trans_sync_def,RTC_RTC]
+QED
+
+(* Basic RTC rules (id) *)
+Theorem trans_sync_one:
+  ∀p τ q. trans p (τ,[]) q ⇒ trans_sync p q
+Proof
+  rw [trans_sync_def] \\ ho_match_mp_tac RTC_SINGLE
+  \\ asm_exists_tac \\ fs []
+QED
+
+(* One can synchronously consume as much of a choreography
+   as needed to perform any tag operation. If the tag
+   does not match anything in the choreography we just
+   consume the whole thing.
+*)
+Theorem Trm_trans:
+  ∀s c τ. no_undefined_vars (s,c) ∧ no_self_comunication c
+   ⇒ trans_sync (s,c) (syncTrm (s,c) τ)
+Proof
+  rw []
+  \\ drule chor_tag_trans \\ rw []
+  \\ rpt (first_x_assum mp_tac)
+  \\ MAP_EVERY Q.SPEC_TAC [(‘τ’,‘τ’),(‘c’,‘c’),(‘s’,‘s’)]
+  \\ ho_match_mp_tac syncTrm_pairind
+  \\ rw [ no_self_comunication_def
+        , no_undefined_vars_def
+        , syncTrm_def
+        , chor_match_def
+        , chor_tl_def
+        , free_variables_def
+        , trans_sync_one
+        , trans_sync_refl
+        , chor_tag_def]
+  \\ TRY (ho_match_mp_tac trans_sync_one \\ asm_exists_tac \\ fs [])
+  \\ ho_match_mp_tac trans_sync_step \\ asm_exists_tac \\ fs []
+  \\ first_x_assum irule \\ rw []
+  \\ TRY (irule chor_tag_trans)
+  \\ fs [no_undefined_vars_def,DELETE_SUBSET_INSERT]
+QED
 
 val _ = export_theory ()
